Organizei os módulos e arquivos

DFA.v
@@ -10,142 +10,144 @@ Definition event := nat.
 
 Module Type DFA.
 
-Parameter states_num_minus_1 : nat.
+  Parameter states_num_minus_1 : nat.
 
-Parameter events_num_minus_1 : nat.
+  Parameter events_num_minus_1 : nat.
 
-Parameter transition : state->event->state.
+  Parameter transition : state->event->state.
 
-Parameter is_marked : state->bool.
+  Parameter is_marked : state->bool.
 
 End DFA.
 
 
 Module DFAUtils (G : DFA).
 
-Definition states_num := S G.states_num_minus_1.
+  Definition states_num := S G.states_num_minus_1.
 
-Definition events_num := S G.events_num_minus_1.
+  Definition events_num := S G.events_num_minus_1.
 
-Definition is_sink_state (q:state) := q >= states_num.
+  Definition is_sink_state (q:state) := q >= states_num.
 
-Definition is_sink_stateb (q:state) := states_num <=? q.
+  Definition is_sink_stateb (q:state) := states_num <=? q.
 
-Definition is_valid_event (e:event) := e <? events_num.
+  Definition is_valid_event (e:event) := e <? events_num.
 
-Fixpoint xtransition q w :=
-  if is_sink_stateb q then states_num else
-    match w with
-      e::w => if is_valid_event e then
-                xtransition (G.transition q e) w
-              else
-                states_num |
-      []  => q
+  Fixpoint xtransition q w :=
+    if is_sink_stateb q then states_num else
+      match w with
+        e::w => if is_valid_event e then
+                  xtransition (G.transition q e) w
+                else
+                  states_num |
+        []  => q
+      end.
+
+  Definition ixtransition := xtransition 0.
+
+  Definition is_tangible q := ~ is_sink_state q /\ exists w, q = ixtransition w.
+
+  Fixpoint transition_list' q events_num :=
+    match events_num with
+      S n => (n, xtransition q [n]) :: transition_list' q n |
+       O  => []
     end.
 
-Definition ixtransition := xtransition 0.
+  Definition transition_list q := transition_list' q events_num.
 
-Fixpoint transition_list' q events_num :=
-  match events_num with
-    S n => (n, xtransition q [n]) :: transition_list' q n |
-     O  => []
-  end.
-
-Definition transition_list q := transition_list' q events_num.
-
-Lemma ixtransition_nil__0 : ixtransition [] = 0.
-Proof.
-  unfold ixtransition.
-  reflexivity.
-Qed.
-
-Definition is_proper_transition q e := ~ is_sink_state (xtransition q [e]).
-
-Definition is_generated w := ~ is_sink_state (ixtransition w).
-
-Lemma is_sink_stateb__is_sink_state : forall q,
-  is_sink_stateb q = true <-> is_sink_state q.
-Proof.
-  intro q.
-  split; intro H.
-  - apply leb_complete, H.
-  - apply leb_correct, H.
-Qed.
-
-Lemma isnt_sink_stateb__isnt_sink_state : forall q,
-  is_sink_stateb q = false <-> ~ is_sink_state q.
-Proof.
-  intro q.
-  split; intro H.
-  - unfold not.
-    intro contra.
-    apply is_sink_stateb__is_sink_state in contra.
-    rewrite H in contra.
-    discriminate contra.
-  - unfold is_sink_state in H.
-    unfold is_sink_stateb.
-    apply leb_iff_conv.
-    apply not_ge in H.
-    apply H.
-Qed.
-
-Lemma first_sink_state : is_sink_stateb states_num = true.
-Proof.
-  apply is_sink_stateb__is_sink_state.
-  unfold is_sink_state.
-  omega.
-Qed.
-
-Lemma xtransition_sink_state : forall w q,
-  is_sink_stateb q = true -> xtransition q w = states_num.
-Proof.
-  intros w q H.
-  destruct w.
-  - simpl. rewrite H. reflexivity.
-  - simpl.
-    rewrite H.
+  Lemma ixtransition_nil__0 : ixtransition [] = 0.
+  Proof.
+    unfold ixtransition.
     reflexivity.
-Qed.
+  Qed.
 
-Theorem xtransition_distr : forall w w' q,
-  xtransition q (w ++ w') = xtransition (xtransition q w) w'.
-Proof.
-  intros w w'.
-  induction w; intro q.
-  - simpl. destruct (is_sink_stateb q) eqn:eq.
-    + pose proof first_sink_state as H.
-      apply xtransition_sink_state with (w:=w') in H.
-      apply xtransition_sink_state with (w:=w') in eq.
-      rewrite eq, H.
+  Definition is_proper_transition q e := ~ is_sink_state (xtransition q [e]).
+
+  Definition is_generated w := ~ is_sink_state (ixtransition w).
+
+  Lemma is_sink_stateb__is_sink_state : forall q,
+    is_sink_stateb q = true <-> is_sink_state q.
+  Proof.
+    intro q.
+    split; intro H.
+    - apply leb_complete, H.
+    - apply leb_correct, H.
+  Qed.
+
+  Lemma isnt_sink_stateb__isnt_sink_state : forall q,
+    is_sink_stateb q = false <-> ~ is_sink_state q.
+  Proof.
+    intro q.
+    split; intro H.
+    - unfold not.
+      intro contra.
+      apply is_sink_stateb__is_sink_state in contra.
+      rewrite H in contra.
+      discriminate contra.
+    - unfold is_sink_state in H.
+      unfold is_sink_stateb.
+      apply leb_iff_conv.
+      apply not_ge in H.
+      apply H.
+  Qed.
+
+  Lemma first_sink_state : is_sink_stateb states_num = true.
+  Proof.
+    apply is_sink_stateb__is_sink_state.
+    unfold is_sink_state.
+    omega.
+  Qed.
+
+  Lemma xtransition_sink_state : forall w q,
+    is_sink_stateb q = true -> xtransition q w = states_num.
+  Proof.
+    intros w q H.
+    destruct w.
+    - simpl. rewrite H. reflexivity.
+    - simpl.
+      rewrite H.
       reflexivity.
-    + reflexivity.
-  - simpl.
-    pose proof first_sink_state as H.
-    apply xtransition_sink_state with (w:=w') in H.
-    destruct (is_sink_stateb q) eqn:eq.
-    + rewrite H. reflexivity.
-    + destruct (is_valid_event a).
-      * apply IHw.
-      * rewrite H. reflexivity.
-Qed.
+  Qed.
 
-Theorem ixtransition_distr : forall w w',
-  ixtransition (w ++ w') = xtransition (ixtransition w) w'.
-Proof.
-  intros w w'.
-  unfold ixtransition.
-  apply xtransition_distr.
-Qed.
+  Theorem xtransition_distr : forall w w' q,
+    xtransition q (w ++ w') = xtransition (xtransition q w) w'.
+  Proof.
+    intros w w'.
+    induction w; intro q.
+    - simpl. destruct (is_sink_stateb q) eqn:eq.
+      + pose proof first_sink_state as H.
+        apply xtransition_sink_state with (w:=w') in H.
+        apply xtransition_sink_state with (w:=w') in eq.
+        rewrite eq, H.
+        reflexivity.
+      + reflexivity.
+    - simpl.
+      pose proof first_sink_state as H.
+      apply xtransition_sink_state with (w:=w') in H.
+      destruct (is_sink_stateb q) eqn:eq.
+      + rewrite H. reflexivity.
+      + destruct (is_valid_event a).
+        * apply IHw.
+        * rewrite H. reflexivity.
+  Qed.
 
-Theorem prefix_closed : forall w w',
-  is_generated (w ++ w') -> is_generated w.
-Proof.
-  unfold is_generated, ixtransition, not.
-  intros w w' H H0.
-  rewrite xtransition_distr in H.
-  apply is_sink_stateb__is_sink_state in H0.
-  apply H, is_sink_stateb__is_sink_state.
-  destruct w'; simpl; rewrite H0; apply first_sink_state.
-Qed.
+  Theorem ixtransition_distr : forall w w',
+    ixtransition (w ++ w') = xtransition (ixtransition w) w'.
+  Proof.
+    intros w w'.
+    unfold ixtransition.
+    apply xtransition_distr.
+  Qed.
+
+  Theorem prefix_closed : forall w w',
+    is_generated (w ++ w') -> is_generated w.
+  Proof.
+    unfold is_generated, ixtransition, not.
+    intros w w' H H0.
+    rewrite xtransition_distr in H.
+    apply is_sink_stateb__is_sink_state in H0.
+    apply H, is_sink_stateb__is_sink_state.
+    destruct w'; simpl; rewrite H0; apply first_sink_state.
+  Qed.
 
 End DFAUtils.
