QSUpperBound.v
@@ -1,0 +1,418 @@
+Require Import Coq.Init.Nat Coq.Lists.List Omega
+  DFA QueueingSystems QSUtils.
+Require BinIntDef.
+Import ListNotations.
+Local Open Scope Z_scope.
+
+
+Module UpperBound (G : QS).
+
+  Include G.
+
+  Include BufferUtils.
+
+  Include DFAUtils.
+
+  Definition n_upper_bounded := forall w, is_generated w -> n0 + count_buffer w <= n.
+
+  Lemma buffer_count_leq_f : forall (f:state->Z),
+    ( f(0%nat) = n0 /\ forall q, is_tangible q -> forall e, is_valid_event e = true ->
+      is_proper_transition q e -> f(xtransition q [e]) >= f(q) + count_event e )
+    -> forall w, is_generated w -> n0 + count_buffer w <= f(ixtransition w).
+  Proof.
+    intros f [H H0] w H1.
+    induction w as [|e w IHw] using @rev_ind.
+    - simpl.
+      rewrite ixtransition_nil__0.
+      omega.
+    - pose H1 as H2; apply prefix_closed in H2.
+      apply IHw in H2.
+      rewrite ixtransition_distr.
+      rewrite count_buffer_distr'.
+      remember (ixtransition w) as q eqn:eq_q.
+      destruct (is_sink_stateb q) eqn:H3. {
+        apply is_sink_stateb__is_sink_state in H3.
+        apply prefix_closed in H1.
+        unfold is_generated in H1.
+        rewrite <- eq_q in H1.
+        contradiction.
+      }
+      remember (xtransition q [e]) as q' eqn:eq_q'.
+      destruct (is_sink_stateb q') eqn:H4. {
+        unfold is_generated in H1.
+        rewrite ixtransition_distr in H1.
+        rewrite <- eq_q, <- eq_q' in H1.
+        apply is_sink_stateb__is_sink_state in H4.
+        contradiction.
+      }
+      assert (f q' >= f q + count_event e). {
+        rewrite eq_q'.
+        apply H0.
+        - split.
+          + apply isnt_sink_stateb__isnt_sink_state in H3.
+            apply H3.
+          + exists w.
+            apply eq_q.
+        - pose eq_q' as H5.
+          unfold xtransition in H5.
+          rewrite H3 in H5.
+          destruct (is_valid_event e).
+          * reflexivity.
+          * apply isnt_sink_stateb__isnt_sink_state in H4.
+            unfold is_sink_state in H4.
+            omega.
+        - unfold is_proper_transition.
+          rewrite <- eq_q'.
+          apply isnt_sink_stateb__isnt_sink_state.
+          apply H4.
+      }
+      omega.
+  Qed.
+
+  Fixpoint verify_upper_bound' (s:list (option Z)) (fuel:nat) (q:state) (m:Z) :=
+  match fuel with O => update s 0 2 | S fuel =>
+
+      if (length s <=? S q)%nat then (* if q is a sink state *)
+          update s 0 0
+      else if optZ_eq (nth (S q) s None) None then
+          foreach (transition_list q)
+                  (verify_upper_bound' (update s (S q) m) fuel)
+                  (fun e => m + count_event e)
+                  max_lists
+                  (Some 0 :: initial_solution states_num)
+      else if optZ_ge (nth (S q) s None) (Some m) then (* if s[q+1] >= m *)
+          update s 0 0
+      else (* if s[q+1] < m *)
+          update s 0 1
+
+  end.
+
+  Definition verify_upper_bound :=
+    let s := verify_upper_bound' (Some 1 :: initial_solution states_num) (S states_num) 0%nat n0 in
+    extract 0 s (all_but_first_le s n).
+
+  (* Theorem vub_never_runs_out_of_fuel :
+    nth 0
+        (verify_upper_bound' (Some 1 :: initial_solution states_num) (S states_num) 0%nat n0)
+        None
+    <> Some 2.
+  Proof.
+  Admitted. *)
+
+  Lemma vub_s0_none : forall q sn o,
+    nth (S q) (Some o::initial_solution sn) None = None.
+  Proof.
+    intros q sn; simpl.
+    induction sn as [|sn IH]. destruct q; try (destruct q); reflexivity.
+    simpl; destruct (q <? length (initial_solution sn))%nat eqn:H.
+    apply Nat.ltb_lt in H. rewrite app_nth1. try (apply IH). apply H.
+    rewrite app_nth2.
+      remember (q - length (initial_solution sn))%nat as n1;
+        destruct n1; try (destruct n1); reflexivity.
+      apply Nat.ltb_ge in H; omega.
+  Qed.
+
+  Lemma vub_s0_length : forall o,
+    length (Some o :: initial_solution states_num) = S states_num.
+  Proof.
+    intro o.
+    induction states_num as [|n1 IHn1]; simpl;
+    try (simpl in IHn1; rewrite app_length; simpl; rewrite Nat.add_1_r;
+    rewrite <- IHn1); reflexivity.
+  Qed.
+
+  Lemma vub_foreach_length' : forall q en s u f,
+    (forall (s : list (option Z)) (q : state) (m : Z),
+        length s = S states_num ->
+        length (verify_upper_bound' s u q m) = length s) ->
+    (length s = S states_num ->
+    length (foreach (transition_list' q en)
+      (verify_upper_bound' s u)
+      f max_lists
+      (Some 0 :: initial_solution states_num)) =
+    length s).
+  Proof.
+    intros q en s u f H0 H.
+    induction en as [|en IH].
+    remember (Some 0 :: initial_solution states_num) as s0;
+      simpl; rewrite Heqs0; rewrite vub_s0_length; auto.
+    simpl; simpl in IH; rewrite max_lists_length;
+    rewrite H0; try (rewrite IH); auto.
+  Qed.
+
+  Lemma vub_length : forall s u q m,
+    length s = S states_num ->
+    length (verify_upper_bound' s u q m) = length s.
+  Proof.
+    intros s u.
+    generalize dependent s.
+    induction u as [|u IH]; intros s q m H. apply update_length.
+    simpl; destruct (length s <=? S q)%nat.
+    2: destruct (optZ_eq (nth (S q) s None)).
+    3: destruct (optZ_ge (nth (S q) s None) (Some m)).
+    1,3-4: apply update_length.
+    rewrite max_lists_length.
+    rewrite IH; rewrite update_length; auto.
+    rewrite IH; rewrite update_length; symmetry.
+    replace (Some 0 :: initial_solution states_num_minus_1 ++ [None])
+      with (Some 0 :: initial_solution states_num).
+    2-3: auto.
+
+    rewrite vub_foreach_length'.
+    apply update_length.
+    apply IH.
+    rewrite <- H; apply update_length.
+  Qed.
+
+  Lemma vub_foreach_length : forall q en s u f,
+    length s = S states_num ->
+    length (foreach (transition_list' q en)
+      (verify_upper_bound' s u)
+      f max_lists
+      (Some 0 :: initial_solution states_num)) =
+    length s.
+  Proof.
+    intros q en s u f H.
+    apply vub_foreach_length'.
+    intros; apply vub_length.
+    1-2: auto.
+  Qed.
+
+  Lemma vub_updated'' : forall i s u a m m' q',
+    length (a :: update s i m) = S states_num ->
+    nth (S i) (verify_upper_bound' (a :: update s i m) u
+      q' m') None = nth (S i) (a :: update s i m) None.
+  Proof.
+    intros i s u.
+    generalize dependent i.
+    generalize dependent s.
+    induction u as [|u IH]; intros s i a m m' q' H. reflexivity.
+    simpl.
+    destruct (length (update s i m) <=? q')%nat eqn:H0. reflexivity.
+    destruct (optZ_eq (nth q' (update s i m) None) None) eqn:H1.
+    destruct (q' =? i)%nat eqn:eq.
+    apply beq_nat_true in eq; rewrite eq, nth_update in H1. discriminate H1.
+      rewrite <- eq; rewrite update_length in H0; apply leb_complete_conv in H0; auto.
+    clear H0; clear H1.
+    2: destruct (optZ_ge (nth q' (update s i m) None) (Some m')); reflexivity.
+    rewrite nth_max_lists. {
+      rewrite update_comm.
+      rewrite IH.
+      2: simpl; rewrite update_length, update_length; simpl in H;
+        rewrite update_length in H; auto.
+      2: apply beq_nat_false; rewrite Nat.eqb_sym; auto.
+      induction events_num_minus_1.
+        simpl; replace (nth i (initial_solution states_num_minus_1 ++ [None]) None) with
+          (nth (S i) (Some 0::initial_solution states_num) None). 2: reflexivity.
+          rewrite vub_s0_none, max_none. apply nth_update_update.
+      simpl.
+      simpl in H; rewrite update_length in H.
+      rewrite nth_max_lists.
+      2:    rewrite vub_foreach_length, vub_length; auto.
+      2,3:  simpl; rewrite update_length, update_length; auto.
+      rewrite IH.
+      2: simpl; rewrite update_length, update_length; auto.
+      rewrite max_distr, max_refl; apply IHn1.
+    }
+    rewrite vub_foreach_length, vub_length; simpl.
+    1-3: simpl in H; rewrite <- update_length with (n:=q')(a0:=m') in H;
+      auto.
+  Qed.
+
+  Lemma vub_updated' : forall q q' a s m en,
+    length s = states_num ->
+    (q < length s)%nat ->
+    nth (S q) (max_lists
+                (verify_upper_bound' (a :: update s q m) (length s)
+                  q' (m + count_event en))
+                (foreach (transition_list' q en)
+                  (verify_upper_bound' (a :: update s q m) (length s))
+                  (fun e : nat => m + count_event e) max_lists
+                  (Some 0 :: initial_solution states_num)))
+    None = Some m.
+  Proof.
+    intros q q' a s m en H H0.
+    generalize dependent q'.
+    induction en as [|en IH]; intro q'. {
+      simpl; rewrite nth_max_lists.
+      2: rewrite vub_s0_length; rewrite vub_length; simpl; rewrite update_length;
+        rewrite H; reflexivity.
+      rewrite vub_updated'';
+      replace (Some 0 :: initial_solution states_num_minus_1 ++ [None])
+        with (Some 0 :: initial_solution states_num); try (rewrite vub_s0_none).
+      simpl; rewrite nth_update.
+      4: simpl; rewrite update_length; apply eq_S.
+      1-5: auto.
+    }
+    simpl;
+    replace (initial_solution states_num_minus_1 ++ [None]) with (initial_solution states_num).
+    2: reflexivity.
+    remember (if is_sink_stateb q then states_num else if is_valid_event en then
+              if is_sink_stateb (transition q en) then states_num else transition q en
+              else states_num) as q''.
+    clear Heqq''.
+    rewrite nth_max_lists.
+    2: rewrite max_lists_length, vub_length, vub_length; auto.
+    4: rewrite vub_length; try (rewrite vub_foreach_length).
+    2-6: simpl; rewrite update_length; rewrite H; reflexivity.
+    rewrite IH, vub_updated''; simpl; apply eq_S in H. rewrite nth_update.
+    simpl; destruct (m >=? m); reflexivity.
+    2: rewrite update_length.
+    1-2: auto.
+  Qed.
+
+  Lemma vub_updated : forall q s s' b m,
+    length s = S states_num ->
+    (S q < length s)%nat ->
+    s' = verify_upper_bound' s (length s) q m ->
+    optZ_eq (nth (S q) s None) None = true ->
+    nth q (fst (extract 0 s' b)) None = Some m.
+  Proof.
+    intros q s s' b m H2 H H0 H1; apply leb_iff_conv in H.
+    pose vub_length as s_s'_length; specialize (s_s'_length s (length s) q m);
+      rewrite <- H0 in s_s'_length.
+    destruct s as [|a s]. apply leb_iff_conv in H; simpl in H; omega.
+    simpl in H; simpl in H1; simpl in H0; rewrite H, H1 in H0;
+    destruct s' as [|a' s']. discriminate s_s'_length.
+    apply H2.
+    rewrite fst_extract;
+    replace (initial_solution states_num_minus_1 ++ [None]) with (initial_solution states_num) in H0.
+    2: reflexivity.
+    apply leb_iff_conv in H; eapply vub_updated' in H.
+    rewrite <- H0 in H; apply H.
+    injection H2; auto.
+  Qed.
+
+  Theorem vub_correct :
+    n_upper_bounded <-> snd verify_upper_bound = true.
+  Proof.
+  Admitted.
+
+  Definition state_upper_bound (q:state) :=
+    match nth q (fst verify_upper_bound) None with
+      Some x => x |
+       None  => n
+    end.
+
+  Lemma tangible_state_upper_bound : n_upper_bounded ->
+    forall q, state_upper_bound q <= n.
+  Proof.
+    intros H q.
+    apply vub_correct in H; unfold verify_upper_bound in H.
+    unfold state_upper_bound, verify_upper_bound.
+    remember (Some 1 :: initial_solution states_num) as s0;
+    remember (verify_upper_bound' s0 (S states_num) 0%nat n0) as s;
+    remember (all_but_first_le s n).
+    destruct s. discriminate H.
+    apply extract_true in H.
+    rewrite fst_extract.
+    simpl in Heqb. rewrite Heqb in H.
+    destruct (nth q s) as [x|] eqn:eq.
+    2: omega.
+    eapply all_le_nth.
+    apply H.
+    apply eq.
+  Qed.
+
+  Lemma q0_upper_bound : state_upper_bound 0%nat = n0.
+  Proof.
+    unfold state_upper_bound, verify_upper_bound.
+    remember (Some 1 :: initial_solution states_num) as s0;
+    remember (verify_upper_bound' s0 (S states_num) 0%nat n0) as s;
+    remember (all_but_first_le s n);
+    clear Heqb.
+    assert (s = verify_upper_bound' s0 (S states_num) 0%nat n0). auto.
+    unfold verify_upper_bound' in Heqs.
+    destruct (length s0 <=? 1)%nat eqn:?H. {
+      rewrite Heqs0, vub_s0_length in H0; unfold states_num in H0; apply leb_complete in H0;
+      omega.
+    }
+    destruct (optZ_eq (nth 1 s0 None) None) eqn:?H.
+    rewrite vub_updated with (m:=n0) (s:=s0).
+    reflexivity.
+    rewrite Heqs0; apply vub_s0_length.
+    apply leb_iff_conv; apply H0.
+    rewrite Heqs0; rewrite vub_s0_length; rewrite <- Heqs0; apply H.
+    apply H1.
+    rewrite Heqs0 in H1; rewrite vub_s0_none in H1; simpl in H1;
+      discriminate H1.
+  Qed.
+
+  Lemma transition_upper_bound : n_upper_bounded ->
+    forall q e, is_tangible q -> is_valid_event e = true -> is_proper_transition q e ->
+    state_upper_bound (xtransition q [e]) >= state_upper_bound q + count_event e.
+  Proof.
+  Admitted.
+
+  Theorem iff_exists_function__upper_bounded :
+    ( exists f, f(0%nat) = n0 /\ forall q, is_tangible q -> 
+       f(q) <= n /\ (forall e, is_valid_event e = true ->
+          is_proper_transition q e -> f(xtransition q [e]) >= f(q) + count_event e ))
+    <-> n_upper_bounded.
+  Proof.
+    split.
+
+    - unfold n_upper_bounded.
+      intros [f [H H0]] w H1.
+      assert (H2: n0 + count_buffer w <= f(ixtransition w)). {
+        apply buffer_count_leq_f; try split; try (apply H); try (apply H0); try (apply H1).
+      }
+      assert (f (ixtransition w) <= n). {
+        destruct (is_sink_stateb (ixtransition w)) eqn:H3.
+        - apply is_sink_stateb__is_sink_state in H3.
+          contradiction.
+        - destruct H0 with (q:=ixtransition w). {
+            split.
+              - apply isnt_sink_stateb__isnt_sink_state.
+                apply H3.
+              - exists w.
+                reflexivity.
+          }
+          apply H4.
+      }
+      omega.
+
+    - intro H.
+      exists state_upper_bound.
+      split.
+      2: intros q H0; split.
+      + apply q0_upper_bound.
+      + apply tangible_state_upper_bound; auto.
+      + intros e H1 H2; apply transition_upper_bound; auto.
+  Qed.
+
+End UpperBound.
+
+
+Module Example.
+
+  Module QS0 <: QS.
+    Definition states_num_minus_1 : nat := 5.
+    Definition events_num_minus_1 : nat := 2.
+    Definition transition (q:state) (e:event) : state :=
+      match q, e with
+        0%nat, 0%nat => 1%nat |
+        1%nat, 0%nat => 2%nat |
+        2%nat, 1%nat => 3%nat |
+        3%nat, 1%nat => 1%nat |
+        0%nat, 2%nat => 4%nat |
+        4%nat, 0%nat => 5%nat |
+        5%nat, 0%nat => 1%nat |
+        _, _=> 6%nat
+      end.
+    Definition is_marked (q:state) := false.
+    Definition count_event (e:event) :=
+      match e with
+        0%nat =>   1%Z  |
+        1%nat => (-1)%Z |
+          _   =>   0%Z
+      end.
+    Definition n := 3.
+    Definition n0 := 0.
+  End QS0.
+
+  Include UpperBound QS0.
+
+  Compute verify_upper_bound.
+
+End Example.
