makefile
@@ -2,6 +2,7 @@ all: compile
 
 compile:
 	@coqc DFA QSUtils
+	@coqc QueueingSystems
 	@find . -name "*.vo.aux" -type f -delete
 
 clear:
